

Chapter 0 : Functions of Several Variables

Author : Ahmed ZEGLAOUI

A Day

1 Generalities

1.1 Definition of a functions of several variables

Let E, F be two sets.

The product $E \times F = \{(x, y) \mid x \in E \text{ and } y \in F\}$.

Definition 1. A relation \mathcal{R} from E to F is a given subset G (or $G_{\mathcal{R}}$) of $E \times F$.

We say that y is the image of x (and x is the pre-image of y) if $(x, y) \in G$.

The inverse relation \mathcal{R}^{-1} of \mathcal{R} is from F to E defined by:

$$y\mathcal{R}^{-1}x \Leftrightarrow x\mathcal{R}y$$

$$G_{\mathcal{R}^{-1}} = s(G_{\mathcal{R}}), \text{ where } s : E \times F \rightarrow F \times E, (x, y) \mapsto (y, x)$$

Definition 2. A function $f : E \rightarrow F$ is a relation from E to F such that:

For each $x \in E$, there exists at most one image $y \in F$.

The domain of f , denoted $\text{Dom}(f)$, is the subset:

$$\text{Dom}(f) = \{x \in E \mid \text{there exists an image of } x\}$$

If $x \in \text{Dom}(f)$, we denote $f(x)$ its image.

When $\text{Dom}(f) = E$, f is called a map from E to F .

The graph of f is:

$$G_f = \{(x, y) \in E \times F \mid x \in \text{Dom}(f) \text{ and } y = f(x)\}$$

If $F = \mathbb{R}$: $f : E \rightarrow \mathbb{R}$ is a real function.

If $F = \mathbb{C}$: $f : E \rightarrow \mathbb{C}$ is a complex function.

Definition 3. Let $n, m \in \mathbb{N}$. A function $\mathbb{R}^n \rightarrow \mathbb{R}^m$ is called a function of n variables:

$$f : \mathbb{R}^n \rightarrow \mathbb{R}^m$$

$$(x_1, \dots, x_n) \mapsto (f_1(x_1, \dots, x_n), \dots, f_m(x_1, \dots, x_n))$$

We denote by f_j the j -th component (or projection Pr_j) of f :

$$f_j : \mathbb{R}^n \rightarrow \mathbb{R}$$

$$(x_1, \dots, x_n) \mapsto f_j(x_1, \dots, x_n)$$

Another way to write it:

$$Pr_j : \mathbb{R}^m \rightarrow \mathbb{R}, \quad \forall j \in \{1, \dots, m\}$$

$$(y_1, y_2, \dots, y_j, \dots, y_m) \mapsto y_j$$

$$f = (f_1, \dots, f_m) = \sum_{j=1}^m f_j e_j \quad \text{where } e_j = (0, 0, \dots, 1, \dots, 0)$$

If $m = 1$, f is a real function.

If $m > 1$, f is a vector function.

The range (or image) of f is the subset of \mathbb{R}^m defined by:

$$\text{range}(f) = \{y \in \mathbb{R}^m \mid \exists x \in \text{Dom}(f), y = f(x)\}$$

Example 1. 1. $\mathcal{L}(\mathbb{R}^n, \mathbb{R}^m)$ - the set of linear maps from \mathbb{R}^n to \mathbb{R}^m - is a subset of $F(\mathbb{R}^n, \mathbb{R}^m)$

where $\mathcal{F}(\mathbb{R}^n, \mathbb{R}^m)$ is the set of all functions from \mathbb{R}^n to \mathbb{R}^m .

2. An affine function:

$$f : \mathbb{R}^n \rightarrow \mathbb{R}^m$$

$$x \mapsto Ax + b$$

where $b \in \mathbb{R}^m$ and $A \in M_{(m,n)}(\mathbb{R})$.

3. For $\mathbb{R}^2 \rightarrow \mathbb{R}$:

$$f(x, y) = \begin{pmatrix} x & y \end{pmatrix} \begin{pmatrix} \alpha \\ \beta \end{pmatrix} = \alpha x + \beta y$$

1.2 Operations on Functions of Several Variables

1) $\forall f, g \in \mathcal{F}(\mathbb{R}^n, \mathbb{R}^m), \forall \alpha, \beta \in \mathbb{R}$

$$\alpha f + \beta g : \mathbb{R}^n \rightarrow \mathbb{R}^m$$

$$x \mapsto \alpha f(x) + \beta g(x)$$

$(\mathcal{F}(\mathbb{R}^n, \mathbb{R}^m); +; \cdot)$ is a vector space.

2) If $f \in \mathcal{F}(\mathbb{R}^n, \mathbb{R}^m)$ and $g \in \mathcal{F}(\mathbb{R}^m, \mathbb{R}^p)$ then:

$$g \circ f \in \mathcal{F}(\mathbb{R}^n, \mathbb{R}^p)$$

$$\mathbb{R}^n \xrightarrow{f} \mathbb{R}^m \xrightarrow{g} \mathbb{R}^p$$

$$x \mapsto f(x) \mapsto g(f(x))$$

3) Let $f, g \in \mathcal{F}(\mathbb{R}^n, \mathbb{R})$ be two scalar functions.

The product $f \cdot g \in \mathcal{F}(\mathbb{R}^n, \mathbb{R})$ defined by:

$$(f \cdot g)(x) = f(x) \cdot g(x), \quad \forall x \in \text{Dom}(f) \cap \text{Dom}(g)$$

If $g(x) \neq 0, \forall x \in \text{Dom}(g)$, then $\frac{1}{g} : x \rightarrow \frac{1}{g(x)}$

$$\text{Dom}\left(\frac{1}{g}\right) = \{x \in \text{Dom}(g) \mid g(x) \neq 0\}$$

and $\frac{f}{g} = f \cdot \left(\frac{1}{g}\right).$

Example 2. 1. A monomial function of degree P is:

$$(x_1, \dots, x_n) \mapsto \alpha x_1^{p_1} x_2^{p_2} \dots x_n^{p_n}$$

$$p_1 + p_2 + \dots + p_n = P$$

2. A homogeneous polynomial of degree P is a finite sum of monomial functions of degree P .

3. A polynomial function is a finite sum of homogeneous polynomial functions.

4. A rational function is the quotient of two polynomial functions.

Definition 4. The graph of a function $f : \mathbb{R}^n \rightarrow \mathbb{R}^m$ is the subset of $\mathbb{R}^n \times \mathbb{R}^m \cong \mathbb{R}^{n+m}$ defined by:

$$G_f = \{(x, y) \in \mathbb{R}^n \times \mathbb{R}^m \mid x \in \text{Dom}(f) \text{ and } y = f(x)\}$$

Remark 1. *If we consider the function:*

$$\tilde{f} : \text{Dom}(f) \rightarrow \mathbb{R}^{n+m}$$

$$x \mapsto (x, f(x))$$

then $\text{range}(\tilde{f}) = G_f$.

\tilde{f} is a parametrization of G_f .

Example 3. 1. *Affine function $f : \mathbb{R} \rightarrow \mathbb{R}$, $x \mapsto ax + b$:*

$$G_f = \{(x, y) \in \mathbb{R}^2 \mid x \in \mathbb{R} \text{ and } y = ax + b\}$$

2. *$f : \mathbb{R}^2 \rightarrow \mathbb{R}$, $(x, y) \mapsto \sqrt{16 - 4x^2 - y^2}$:*

$$\text{Dom}(f) = \{(x, y) \in \mathbb{R}^2 \mid 4x^2 + y^2 \leq 16\}$$

$$\text{range}(f) = \{z \in \mathbb{R} \mid \exists (x, y) \in \text{Dom}(f), z = \sqrt{16 - 4x^2 - y^2}\}$$

Since $4x^2 + y^2 \geq 0$, we have:

$$0 \leq 16 - 4x^2 - y^2 \leq 16 \Rightarrow 0 \leq \sqrt{16 - 4x^2 - y^2} \leq 4$$

Thus $\text{range}(f) = [0, 4]$.

The graph is:

$$G_f = \left\{ (x, y, z) \in \mathbb{R}^3 \mid (x, y) \in \text{Dom}(f) \text{ and } \begin{cases} z^2 + 4x^2 + y^2 = 16 \\ z \geq 0 \end{cases} \right\}$$

2 Limits and Continuity

2.1 Limits

Definition 5. *Let $f : \mathbb{R}^n \rightarrow \mathbb{R}$, $l \in \mathbb{R}$, and $a \in \mathbb{R}^n$.*

$$\lim_{x \rightarrow a} f(x) = l$$

$$\Leftrightarrow \forall \epsilon > 0, \exists \delta > 0, \forall x \in \text{Dom}(f); 0 < d(x, a) < \delta \implies |f(x) - l| < \epsilon$$

$$\lim_{x \rightarrow a} f(x) = +\infty \text{ (resp. } -\infty)$$

$$\Leftrightarrow \forall \alpha > 0, \exists \delta > 0, \forall x \in \text{Dom}(f); 0 < d(x, a) < \delta \implies f(x) > \alpha \text{ (resp. } f(x) < -\alpha)$$

where $d : \mathbb{R}^n \times \mathbb{R}^n \rightarrow \mathbb{R}_+$ is one of the following distances:

Euclidean distance:

$$d_2((x_1, \dots, x_n), (y_1, \dots, y_n)) = \sqrt{\sum_{i=1}^n (y_i - x_i)^2}$$

Manhattan distance:

$$d_1((x_1, \dots, x_n), (y_1, \dots, y_n)) = \sum_{i=1}^n |y_i - x_i|$$

Chebyshev distance:

$$d_\infty((x_1, \dots, x_n), (y_1, \dots, y_n)) = \max_{1 \leq i \leq n} |y_i - x_i|$$

Remark 2. If $n = 1$, then $d_1 = d_2 = d_\infty$.

Proposition 1.

$$\lim_{x \rightarrow a} f(x) = l \Leftrightarrow \forall (x_n) \subset \text{Dom}(f), \lim_{n \rightarrow +\infty} x_n = a \Rightarrow \lim_{n \rightarrow \infty} f(x_n) = l$$

Remark 3. If the limit l exists, it is unique.

Definition 6. Let $f = (f_1, \dots, f_m) : \mathbb{R}^n \rightarrow \mathbb{R}^m$

$$x \mapsto (f_1(x), \dots, f_m(x))$$

$$\forall j \in \{1, \dots, m\}, \quad l_j = \lim_{x \rightarrow a} f_j(x)$$

If $\forall j; l_j \in \mathbb{R}$, then $\lim_{x \rightarrow a} f(x) = l = (l_1, \dots, l_m) \in \mathbb{R}^m$.

If $\exists j; l_j = \pm\infty$, then $\lim_{x \rightarrow a} f(x)$ does not exist.

Definition 7. $f = (f_1, \dots, f_m) : \mathbb{R}^n \rightarrow \mathbb{R}^m$ is continuous at a point $a \in \text{Dom}(f)$ if:

$$\lim_{x \rightarrow a} f(x) = f(a)$$

Example 4. f continuous at $x = a$

$$\Leftrightarrow \forall (x_n) \subset \text{Dom}(f), \lim_{n \rightarrow +\infty} x_n = a \Rightarrow \lim_{n \rightarrow +\infty} f(x_n) = f(a)$$

Remark 4. To prove that $\lim_{x \rightarrow a} f(x)$ does not exist:

1st method:

We can give two sequences $(x_n), (y_n)$ from $\text{Dom}(f)$ that converge to a

$$\begin{cases} \lim_{n \rightarrow \infty} x_n = a \\ \lim_{n \rightarrow \infty} y_n = a \end{cases}$$

and $\lim_{n \rightarrow +\infty} f(x_n) \neq \lim_{n \rightarrow +\infty} f(y_n)$.

2nd method:

We give two paths (continuous maps $[0, \delta) \rightarrow \text{Dom}(f)$) on $\text{Dom}(f)$ with $\gamma(0) = a$

$$\begin{cases} \gamma_1 : [0, \delta_1) \rightarrow \text{Dom}(f), \gamma_1(0) = a \\ \gamma_2 : [0, \delta_2) \rightarrow \text{Dom}(f), \gamma_2(0) = a \end{cases}$$

If $\lim_{t \rightarrow 0^+} f(\gamma_1(t)) \neq \lim_{t \rightarrow 0^+} f(\gamma_2(t))$, then the limit does not exist.

Example 5. Consider $f(x, y) = \frac{x^2 - y^2}{x^2 + y^2}$.

$$\begin{cases} \gamma_1 : [0, +\infty) \rightarrow \mathbb{R}^2 \\ t \mapsto (t, 0) \end{cases}$$

$$\begin{cases} \gamma_2 : [0, +\infty) \rightarrow \mathbb{R}^2 \\ t \mapsto (0, t) \end{cases}$$

$$f(\gamma_1(t)) = \frac{t^2 - 0^2}{t^2 + 0^2} = 1$$

$$f(\gamma_2(t)) = \frac{0^2 - t^2}{0^2 + t^2} = -1$$

Since $\lim_{t \rightarrow 0^+} f(\gamma_1(t)) \neq \lim_{t \rightarrow 0^+} f(\gamma_2(t))$, the limit does not exist.

Properties:

1) The Linearity:

$$\lim_{x \rightarrow a} f(x) = l_1 \in \mathbb{R}^m \text{ and } \lim_{x \rightarrow a} g(x) = l_2 \in \mathbb{R}^m$$

$$\text{then } \forall \alpha, \beta \in \mathbb{R}, \lim_{x \rightarrow a} [\alpha f(x) + \beta g(x)] = \alpha l_1 + \beta l_2$$

2) Limit of Product and quotient

$$f \times g : \mathbb{R}^n \rightarrow \mathbb{R}$$

$$\text{If } \lim_{x \rightarrow a} f(x) = l_1 \text{ and } \lim_{x \rightarrow a} g(x) = l_2$$

$$\text{Then } \lim_{x \rightarrow a} (fg)(x) = l_1 l_2$$

$$\text{And if } g(x) \neq 0, \lim_{x \rightarrow a} \frac{f(x)}{g(x)} = \frac{l_1}{l_2}$$

3) Limit of Composed functions

$$\text{If } f : \mathbb{R}^n \rightarrow \mathbb{R}^m \text{ continuous at } a \text{ and } \lim_{y \rightarrow f(a)} g(y) = l$$

$$\text{then } \lim_{x \rightarrow a} (g \circ f)(x) = l$$

Definition 8. 1) Let $f : \mathbb{R}^n \rightarrow \mathbb{R}$ and $\emptyset \neq V \subset \text{Dom}(f)$.

We say that f is continuous on V if:

$$\forall (x_n) \subset V, (x_n) \rightarrow x \in \text{Dom}(f) \implies \lim_{n \rightarrow +\infty} f(x_n) = f(x)$$

$$2) f = (f_1, \dots, f_m) : \mathbb{R}^n \rightarrow \mathbb{R}^m \text{ continuous on } V \subset \text{Dom}(f) = \bigcap_{j=1}^m \text{Dom}(f_j)$$

$$\Leftrightarrow \forall j \in \{1, 2, \dots, m\}, f_j : \mathbb{R}^n \rightarrow \mathbb{R} \text{ is continuous on } V$$

2.2 The Case of $f : \mathbb{R}^2 \rightarrow \mathbb{R}$

Euclidian distance

$$d_1((x_1, x_2), (y_1, y_2)) = |y_1 - x_1| + |y_2 - x_2|$$

$$d_2((x_1, x_2), (y_1, y_2)) = \sqrt{(y_1 - x_1)^2 + (y_2 - x_2)^2}$$

$$d_\infty((x_1, x_2), (y_1, y_2)) = \max(|y_1 - x_1|, |y_2 - x_2|)$$

limit:

$$\lim_{(x,y) \rightarrow (a,b)} f(x,y) = l \quad / l \in \mathbb{R}$$

$$\Leftrightarrow \forall \epsilon > 0, \exists \delta > 0; 0 < d((x,y), (a,b)) < \delta \implies |f(x,y) - l| < \epsilon$$

Example:

$$f(x, y) = \frac{x^3}{x^2 + y^2}$$

$$\lim_{(x,y) \rightarrow (0,0)} f(x, y) = 0$$

$$|f(x, y)| = \left| \frac{x^3}{x^2 + y^2} \right| = |x| \frac{x^2}{x^2 + y^2} \leq |x| \leq |x| + |y| = d_1((x, y), (0, 0))$$

$$\Leftrightarrow \forall \epsilon > 0, \exists \delta = \epsilon > 0, \forall (x, y) \in \mathbb{R}^2 - \{(0, 0)\}, \quad 0 < |x| + |y| < \delta \implies |f(x, y)| < \epsilon$$

Using polar coordinates:

$$\text{Let: } \begin{cases} x = a + r \cos \theta & ; \theta \in \mathbb{R} \\ y = b + r \sin \theta & r > 0 \end{cases}$$

$$d_2((x, y), (a, b)) = \sqrt{(x - a)^2 + (y - b)^2} = \sqrt{(r \cos \theta)^2 + (r \sin \theta)^2} = r$$

$$l \in \overline{\mathbb{R}} = \mathbb{R} \cup \{-\infty, \infty\}$$

$$\lim_{(x,y) \rightarrow (a,b)} f(x, y) = l$$

$$\Leftrightarrow \forall \epsilon > 0, \exists \delta > 0, 0 < r < \delta \implies |f(a + r \cos \theta, b + r \sin \theta) - l| < \epsilon$$

$$\Leftrightarrow \forall \theta \in \mathbb{R}; \lim_{r \rightarrow 0^+} f(a + r \cos \theta, b + r \sin \theta) = l$$

Example:

$$f(x, y) = \frac{x^2 - y^2}{x^2 + y^2}, \quad (a, b) = (0, 0)$$

$$f(a + r \cos \theta, b + r \sin \theta) = \frac{r^2 \cos^2 \theta - r^2 \sin^2 \theta}{r^2 \cos^2 \theta + r^2 \sin^2 \theta} = \cos^2 \theta - \sin^2 \theta$$

$$\theta = 0, l = 1$$

$$\theta = \frac{\pi}{2}, l = -1$$

\implies limit does not exist.

Example 2:

$$f(x, y) = \frac{x^3 + y^3}{x^2 + y^2}$$

$$f(r \cos \theta, r \sin \theta) = \frac{r^3(\cos^3 \theta + \sin^3 \theta)}{r^2} = r(\cos^3 \theta + \sin^3 \theta)$$

$$0 \leq |f(r \cos \theta, r \sin \theta)| = r|\cos^3 \theta + \sin^3 \theta| \leq 2r \rightarrow 0$$

$$\text{So } \lim_{(x,y) \rightarrow (0,0)} \frac{x^3 + y^3}{x^2 + y^2} = 0$$

2.3 The Case of $f : \mathbb{R}^3 \rightarrow \mathbb{R}$

$$\lim_{(x,y,z) \rightarrow (x_0,y_0,z_0)} f(x,y,z) = l$$

Using cylindrical coordinates:

$$\begin{cases} x = x_0 + r \cos \theta & ; r > 0 \\ y = y_0 + r \sin \theta & \theta \in \mathbb{R} \\ z = z_0 \end{cases}$$

$$d_2((x,y,z), (x_0,y_0,z_0)) = \sqrt{(x-x_0)^2 + (y-y_0)^2 + (z-z_0)^2} = \sqrt{r^2 + (z-z_0)^2}$$

We note $g_\theta = f(x_0 + r \cos \theta, y_0 + r \sin \theta, z)$

$$\forall \epsilon > 0; \exists \delta > 0; d_2((r,z), (0,z_0)) < \delta \implies |g_\theta(r,z) - l| < \epsilon$$

$$\begin{aligned} & \lim_{(x,y,z) \rightarrow (x_0,y_0,z_0)} f(x,y,z) = l \\ \Leftrightarrow & \forall \theta \in \mathbb{R}, \lim_{(r,z) \rightarrow (0,z_0)} g_\theta(r,z) = l \end{aligned}$$

Example:

$$\begin{aligned} f(x,y,z) &= \frac{x^2 + y^2 - z^2}{x^2 + y^2 + z^2} \\ g_\theta(r,z) &= \frac{r^2 - z^2}{r^2 + z^2} \end{aligned}$$

Since $\lim_{(r,z) \rightarrow (0,0)} g_\theta(r,z)$ does not exist, then $\lim_{(x,y,z) \rightarrow (0,0,0)} \frac{x^2 + y^2 - z^2}{x^2 + y^2 + z^2}$ does not exist.

Using spherical coordinates:

$$\begin{cases} x = x_0 + r \cos \theta \cos \varphi \\ y = y_0 + r \cos \theta \sin \varphi \\ z = z_0 + r \sin \theta \end{cases}$$

$$g_{\theta,\varphi}(r) = f(x,y,z)$$

$$d_2((x,y,z), (x_0,y_0,z_0)) = r$$

So;

$$\begin{aligned} & \lim_{(x,y,z) \rightarrow (x_0,y_0,z_0)} f(x,y,z) = l \\ \Leftrightarrow & \forall \theta, \varphi, \lim_{r \rightarrow 0^+} g_{\theta,\varphi}(r) = l \end{aligned}$$

Example:

$$f(x, y, z) = \frac{x^2 + y^2 - z^2}{x^2 + y^2 + z^2}$$

Since $\lim_{r \rightarrow 0^+} g_{\theta, \varphi}(r)$ depends on θ and φ , the limit does not exist.

3 differentiation

3.1 First partial derivatives

The process of "partial differentiation" consists of deriving a function of several variables with respect to one of its independent variables.

The result is referred to as the "partial derivative of f with respect to the chosen independent variable.

Definition 9. Let $f : \mathbb{R}^2 \rightarrow \mathbb{R}; \quad (a, b) \in \text{Dom}(f)$

1) If the limit $\lim_{h \rightarrow 0} \frac{f(a+h, b) - f(a, b)}{h} \in \mathbb{R}$ exists, we call it the first partial derivative of f with respect to the first independent variable x , denoted by: $\frac{\partial f}{\partial x}(a, b)$

2) If the limit $\lim_{h \rightarrow 0} \frac{f(a, b+h) - f(a, b)}{h} \in \mathbb{R}$ exists, we call it the first partial derivative of f at (a, b) with respect to the second independent variable, denoted by: $\frac{\partial f}{\partial y}(a, b)$

3) We define two functions, $f_x = \frac{\partial f}{\partial x}$ and $\frac{\partial f}{\partial y}$ by:

$$\begin{aligned} f_x &= \frac{\partial f}{\partial x} : \mathbb{R}^2 \rightarrow \mathbb{R} \\ (x, y) &\mapsto \frac{\partial f}{\partial x}(x, y) = \lim_{h \rightarrow 0} \frac{f(x+h, y) - f(x, y)}{h} \\ f_y &= \frac{\partial f}{\partial y} : \mathbb{R}^2 \rightarrow \mathbb{R} \\ (x, y) &\mapsto \frac{\partial f}{\partial y}(x, y) = \lim_{h \rightarrow 0} \frac{f(x, y+h) - f(x, y)}{h} \end{aligned}$$

example:

1) $f(x, y) = \phi(x)\psi(y)$

$$\frac{\partial f}{\partial x}(x, y) = \phi'(x)\psi(y)$$

$$\frac{\partial f}{\partial y}(x, y) = \phi(x)\psi'(y)$$

Geometric Interpretation

The tangent line of the curve $z = f(x, b)$ at $(a, f(a, b))$ is directed by $(1, 0, \frac{\partial f}{\partial x}(a, b))$

$$\begin{cases} z = f(a, b) + (x - a)\frac{\partial f}{\partial x}(a, b) \\ y = b \end{cases}$$

The tangent line of the curve $z = f(a, y)$ at $(a, b, f(a, b))$ is directed by $(0, 1, \frac{\partial f}{\partial y}(a, b))$

$$\begin{cases} z = f(a, b) + (y - b)\frac{\partial f}{\partial y}(a, b) \\ x = a \end{cases}$$

The tangent plane of the graph of f at $(a, b, f(a, b))$, denoted by $T_{(a,b,f(a,b))}G_f$ is defined by

$$T_{(a,b,f(a,b))}G_f = \{(x, y, z) \in \mathbb{R}^3 : z = f(a, b) + \frac{\partial f}{\partial x}(a, b)(x - a) + \frac{\partial f}{\partial y}(a, b)(y - b)\}$$

Definition 10. 1) Let

$$f : \mathbb{R}^n \rightarrow \mathbb{R}$$

$$(x_1, \dots, x_n) \mapsto f(x_1, \dots, x_n)$$

$$\forall i \in \{1, 2, \dots, n\}, \quad f_{x_i} = \frac{\partial f}{\partial x_i} : \mathbb{R}^n \rightarrow \mathbb{R}$$

$$(x_1, \dots, x_n) \mapsto \frac{\partial f}{\partial x_i}(x_1, \dots, x_n) = \lim_{h \rightarrow 0} \frac{f(x_1, \dots, x_i + h, \dots, x_n) - f(x_1, \dots, x_n)}{h}$$

$\frac{\partial f}{\partial x_i}$ is the i -th first derivative of f or the first partial derivative of f with respect to the i -th independent variable.

When $m > 1$: $f = (f_1, \dots, f_m) : \mathbb{R}^n \rightarrow \mathbb{R}^m$

$$\forall i \in \{1, \dots, m\}; \quad \frac{\partial f}{\partial x_i} = \left(\frac{\partial f_1}{\partial x_i}, \dots, \frac{\partial f_m}{\partial x_i} \right) : \mathbb{R}^n \rightarrow \mathbb{R}^m$$

The tangent plane of $G_f = \{(x, y) \in \mathbb{R}^n \times \mathbb{R}^m : y = f(x)\}$ at $(a, f(a))$, denoted by $T_{(a,f(a))}G_f$ is:

$$T_{(a,f(a))}G_f = \{(x, y) \in \mathbb{R}^n \times \mathbb{R}^m : y = f(a) + \sum_{i=1}^n (x_i - a_i) \frac{\partial f}{\partial x_i}(a)\} \subset \mathbb{R}^{n+m}$$

Example:1

$$f : \mathbb{R}^3 \rightarrow \mathbb{R}, \quad (x, y, z) \mapsto xy + yz^2 + xz$$
$$\frac{\partial f}{\partial x} = y + z, \quad \frac{\partial f}{\partial y} = x + z^2, \quad \frac{\partial f}{\partial z} = 2yz + x$$

3.2 Second Order Partial Derivatives

Definition 11. 1) Let $f : \mathbb{R}^2 \rightarrow \mathbb{R}$ and $\frac{\partial f}{\partial x}, \frac{\partial f}{\partial y}$ its first partial derivatives:

$$f_{xx} = \frac{\partial^2 f}{\partial x^2} = \frac{\partial}{\partial x} \left(\frac{\partial f}{\partial x} \right) (x, y) = \lim_{h \rightarrow 0} \frac{\frac{\partial f}{\partial x}(x+h, y) - \frac{\partial f}{\partial x}(x, y)}{h}$$
$$f_{xy} = \frac{\partial^2 f}{\partial y \partial x} = \frac{\partial}{\partial y} \left(\frac{\partial f}{\partial x} \right) (x, y) = \lim_{h \rightarrow 0} \frac{\frac{\partial f}{\partial x}(x, y+h) - \frac{\partial f}{\partial x}(x, y)}{h}$$
$$f_{yx} = \frac{\partial^2 f}{\partial x \partial y} = \frac{\partial}{\partial x} \left(\frac{\partial f}{\partial y} \right) (x, y) = \lim_{h \rightarrow 0} \frac{\frac{\partial f}{\partial y}(x+h, y) - \frac{\partial f}{\partial y}(x, y)}{h}$$
$$f_{yy} = \frac{\partial^2 f}{\partial y^2} = \frac{\partial}{\partial y} \left(\frac{\partial f}{\partial y} \right) (x, y) = \lim_{h \rightarrow 0} \frac{\frac{\partial f}{\partial y}(x, y+h) - \frac{\partial f}{\partial y}(x, y)}{h}$$

2) Let $f : \mathbb{R}^n \rightarrow \mathbb{R}$ and $\frac{\partial f}{\partial x_i}; i \in \{1, \dots, n\}$ its first partial derivatives.

$$\forall i, j \in \{1, \dots, n\}$$

$$\frac{\partial^2 f}{\partial x_i \partial x_j}(x_1, \dots, x_n) = \lim_{h \rightarrow 0} \frac{\frac{\partial f}{\partial x_j}(x_1, \dots, x_i+h, \dots, x_n) - \frac{\partial f}{\partial x_j}(x_1, \dots, x_n)}{h}$$

When $i = j$, $\frac{\partial^2 f}{\partial x_i \partial x_j} = \frac{\partial^2 f}{\partial x_i^2}$ is called the second partial derivative of f with respect to x_i .

When $i \neq j$, $\frac{\partial^2 f}{\partial x_i \partial x_j}$ is called the mixed second partial derivative of f with respect to x_i and x_j .

There are n^2 second partial derivatives of f .

3) If $f = (f_1, \dots, f_m) : \mathbb{R}^n \rightarrow \mathbb{R}^m$

$$\forall i, j \in \{1, \dots, n\}; \frac{\partial^2 f}{\partial x_i \partial x_j} = \left(\frac{\partial^2 f_1}{\partial x_i \partial x_j}, \dots, \frac{\partial^2 f_m}{\partial x_i \partial x_j} \right)$$

Theorem 1 (Schwarz's Theorem). *Let $f : \mathbb{R}^n \rightarrow \mathbb{R}^m$.*

If $\frac{\partial^2 f}{\partial x_i \partial x_j}$ and $\frac{\partial^2 f}{\partial x_j \partial x_i}$ are continuous on an open subset $D \subset \mathbb{R}^n$, then

$$\frac{\partial^2 f}{\partial x_i \partial x_j} = \frac{\partial^2 f}{\partial x_j \partial x_i} \quad \text{on } D$$

Definition 12. Higher order partial derivatives

Let $p \in \mathbb{N}^$; $f : \mathbb{R}^n \rightarrow \mathbb{R}^m$. The p -th partial derivatives of f are :*

$$\frac{\partial^p f}{\partial x_{i_1} \partial x_{i_2} \dots \partial x_{i_{p-1}} \partial x_{i_p}} := \frac{\partial}{\partial x_{i_1}} \left(\frac{\partial}{\partial x_{i_2}} \left(\dots \left(\frac{\partial f}{\partial x_{i_{p-1}}} \left(\frac{\partial f}{\partial x_{i_p}} \right) \right) \right) \right), \quad \text{where } i_1, i_2, \dots, i_p \in \{1, 2, \dots, n\}$$

Definition 13. 1) *We say that a function is C^1 (of class C^1) if all its first partial derivatives are continuous.*

2) *We say that a function is of class C^p if all its partial derivatives of degree p are continuous.*

3) *We say that a function is C^∞ if all partial derivatives of degree p exist; $\forall p \in \mathbb{N}$.*

Corollary

If f is of class C^p , all the p -th partial derivatives can be written as

$$\frac{\partial^p f}{\partial x_1^{p_1} \partial x_2^{p_2} \dots \partial x_n^{p_n}} \quad \forall p_1, \dots, p_n \in \mathbb{N} \text{ such that } p_1 + p_2 + \dots + p_n = p$$

Example:

If $f : \mathbb{R}^2 \rightarrow \mathbb{R}$ is of class C^3 , the third partials derivatives are of the form: $\frac{\partial^3 f}{\partial x^p \partial y^q}$
where $p + q = 3$

$$\begin{aligned} \frac{\partial^3 f}{\partial x^3}, \quad \frac{\partial^3 f}{\partial y^3} \\ \frac{\partial^3 f}{\partial x^2 \partial y} = \frac{\partial^3 f}{\partial x \partial y \partial x} = \frac{\partial^3 f}{\partial y \partial x^2} \\ \frac{\partial^3 f}{\partial y^2 \partial x} = \frac{\partial^3 f}{\partial y \partial x \partial y} = \frac{\partial^3 f}{\partial x \partial y^2} \end{aligned}$$

3.3 Differentials of a Function

Recall that if

$$f : \mathbb{R} \rightarrow \mathbb{R}, \quad x \mapsto f(x)$$

is derivable function and f' is its derivative function, then the differential of f , denoted df , is the function

$$df : \mathbb{R} \rightarrow \mathcal{L}(\mathbb{R}, \mathbb{R}) = \{\phi : \mathbb{R} \rightarrow \mathbb{R} \mid \phi \text{ linear}\}$$

$$x \mapsto d_x f : \mathbb{R} \rightarrow \mathbb{R}, \quad h \mapsto f'(x) \cdot h$$

Definition 14. Let $f : \mathbb{R}^n \rightarrow \mathbb{R}^m$ be a function such that all first partial derivatives exist.

Then the differential of f is the function

$$df : \mathbb{R}^n \rightarrow \mathcal{L}(\mathbb{R}^n, \mathbb{R}^m)$$

$$x \mapsto d_x f : \mathbb{R}^n \rightarrow \mathbb{R}^m, \quad h = (h_1, \dots, h_n) \mapsto \sum_{i=1}^n h_i \frac{\partial f}{\partial x_i}(x)$$

Remark: If $f : \mathbb{R}^n \rightarrow \mathbb{R}^m$ is linear, then:

$$\forall x \in \mathbb{R}^n : \quad d_x f = f$$

In Particular: $f = \text{pr}_i : (x_1, \dots, x_n) \mapsto x_i$

$$\forall x, d_x f = f = \text{pr}_i = dx_i : \mathbb{R}^n \rightarrow \mathbb{R}, \quad (h_1, \dots, h_n) \mapsto h_i$$

If $m = 1$:

$$d_x f = \sum_{i=1}^n \frac{\partial f}{\partial x_i}(x) dx_i$$

Example:

$$f : \mathbb{R}^2 \rightarrow \mathbb{R}, \quad (x, y) \mapsto f(x, y)$$

$$d_{(x,y)} f = \frac{\partial f}{\partial x}(x, y) dx + \frac{\partial f}{\partial y}(x, y) dy$$

$$df = \frac{\partial f}{\partial x} dx + \frac{\partial f}{\partial y} dy$$

$$f(x, y) = xy; \quad d_{(x,y)} f = y dx + x dy$$

Application: $w = f(x_1, \dots, x_n); \Delta w = f(x_1 + \Delta x_1, \dots, x_n + \Delta x_n) - f(x_1, \dots, x_n)$

Then:

$$\Delta w \approx \sum_{i=1}^n \frac{\partial f}{\partial x_i}(x_1, \dots, x_n) \Delta x_i$$

Definition 15. Differentiability

Let $f : \mathbb{R}^n \rightarrow \mathbb{R}^m$, and $a \in \mathbb{R}^n$

We say that f is differentiable at a if there exists a linear map

$$\mathcal{L}_a : \mathbb{R}^n \rightarrow \mathbb{R}^m, \quad h \mapsto \mathcal{L}_a(h)$$

such that:

$$\lim_{h \rightarrow 0_{\mathbb{R}^n}} \frac{1}{\|h\|} (f(a+h) - f(a) - \mathcal{L}_a(h)) = 0$$

where $\|h\| = \sqrt{h_1^2 + \dots + h_n^2}$.

Remark: If f is differentiable at (a_1, \dots, a_n) , then:

$\forall i \in \{1, \dots, n\}$, if we consider $h = (0, \dots, 0, t, 0, \dots, 0) = te_i$

$$\begin{aligned} \lim_{t \rightarrow 0} \frac{1}{|t|} (f(a + te_i) - f(a) - \mathcal{L}_a(te_i)) &= 0 \\ \Rightarrow \lim_{t \rightarrow 0} \frac{1}{t} (f(a + te_i) - f(a)) &= \mathcal{L}_a(e_i) \\ \Rightarrow \frac{\partial f}{\partial x_i}(a) &= \mathcal{L}_a(e_i) \quad \forall i \in \{1, \dots, n\} \end{aligned}$$

$$\mathcal{L}_a(h) = \mathcal{L}_a\left(\sum_{i=1}^n h_i e_i\right) = \sum_{i=1}^n h_i \mathcal{L}_a(e_i) = \sum_{i=1}^n h_i \frac{\partial f}{\partial x_i}(a) = d_a f(h)$$

So, $\mathcal{L}_a = d_a f$.

Thus, f is differentiable at a if and only if all its first partial derivatives exist and

$$f(a+h) = f(a) + d_a f(h) + o(\|h\|)$$

where $\lim_{h \rightarrow 0_{\mathbb{R}^n}} \frac{1}{\|h\|} o(\|h\|) = 0$.

Proposition:

If $f : \mathbb{R}^n \rightarrow \mathbb{R}^m$ is differentiable at a , then f is continuous at a .

Proof: By the relation:

$$f(a+h) - f(a) = d_a f(h) + \|h\| \epsilon(h)$$

where $\lim_{h \rightarrow 0_{\mathbb{R}^n}} \epsilon(h) = 0$. Since $d_a f$ is a linear map, it is continuous, then:

$$\lim_{h \rightarrow 0_{\mathbb{R}^n}} [f(a+h) - f(a)] = 0 \Leftrightarrow \lim_{x \rightarrow a} f(x) = f(a)$$

Example:

$$f(x, y) = \begin{cases} \frac{xy^2}{x^2 + y^2} & \text{if } (x, y) \neq (0, 0) \\ 0 & \text{if } (x, y) = (0, 0) \end{cases}$$

f is continuous at $(0, 0)$, because:

$$|f(x, y)| = |x| \left(\frac{y^2}{x^2 + y^2} \right) \leq |x| \xrightarrow{(x, y) \rightarrow (0, 0)} 0$$

So $\lim_{(x, y) \rightarrow (0, 0)} f(x, y) = f(0, 0)$.

Now check differentiability:

$$\begin{aligned} \frac{\partial f}{\partial x}(0, 0) &= \lim_{h \rightarrow 0} \frac{f(h, 0) - f(0, 0)}{h} = 0 \\ \frac{\partial f}{\partial y}(0, 0) &= \lim_{h \rightarrow 0} \frac{f(0, h) - f(0, 0)}{h} = 0 \\ &\implies d_{(0,0)} f(h_1, h_2) = 0, \quad \forall (h_1, h_2) \in \mathbb{R}^2 \\ &\lim_{(h_1, h_2) \rightarrow (0, 0)} \frac{f(0 + h_1, 0 + h_2) - f(0, 0) - d_{(0,0)} f(h_1, h_2)}{\sqrt{h_1^2 + h_2^2}} \\ &= \lim_{(h_1, h_2) \rightarrow (0, 0)} \frac{\frac{h_1 h_2^2}{h_1^2 + h_2^2}}{\sqrt{h_1^2 + h_2^2}} \\ &= \lim_{(h_1, h_2) \rightarrow (0, 0)} \frac{h_1 h_2^2}{(h_1^2 + h_2^2)^{3/2}} \end{aligned}$$

This limit does not exist because along $\gamma : t \mapsto (t, t)$:

$$\frac{t \cdot t^2}{(t^2 + t^2)^{3/2}} = \frac{t^3}{(2t^2)^{3/2}} = \frac{t^3}{2\sqrt{2}|t|^3} \rightarrow \frac{1}{2\sqrt{2}} \neq 0$$

So f is not differentiable at $(0, 0)$.

Remark:

If all the first partial derivatives are continuous, then the function is differentiable.

Proposition

Linear combination, product, quotient, composition of functions of class C^p ($p \in \mathbb{N} \cup \{\infty\}$) are of Class C^p .

Theorem 2. Let $f : \mathbb{R}^n \rightarrow \mathbb{R}^m$ differentiable at a and $g : \mathbb{R}^m \rightarrow \mathbb{R}^l$ differentiable at $f(a)$, then :

$$\begin{aligned} g \circ f : \mathbb{R}^n &\xrightarrow{f} \mathbb{R}^m \xrightarrow{g} \mathbb{R}^l \\ x &\mapsto f(x) \mapsto g(f(x)) \end{aligned}$$

is differentiable at a and :

$$\begin{aligned} d_a(g \circ f) &= d_{f(a)}g \circ d_af \\ d_a(g \circ f)(h) &= d_{f(a)}g(d_af(h)) \quad \forall h \in \mathbb{R}^n \end{aligned}$$

Definition 16. *Jacobian matrix - Hessian matrix*

1) Let $f : \mathbb{R}^n \rightarrow \mathbb{R}^m$, $x \mapsto (f_1(x), \dots, f_m(x))$ differentiable at a , the Jacobian matrix of f at a , denoted by $Jac_a(f)$ is the matrix associated with the linear map $d_af : \mathbb{R}^n \rightarrow \mathbb{R}^m$ with respect to the usual bases of \mathbb{R}^n and \mathbb{R}^m :

$$\begin{aligned} Jac_a(f) &= \begin{pmatrix} \frac{\partial f_1}{\partial x_1}(a) & \frac{\partial f_1}{\partial x_2}(a) & \dots & \frac{\partial f_1}{\partial x_n}(a) \\ \frac{\partial f_2}{\partial x_1}(a) & \frac{\partial f_2}{\partial x_2}(a) & \dots & \frac{\partial f_2}{\partial x_n}(a) \\ \vdots & \vdots & \ddots & \vdots \\ \frac{\partial f_m}{\partial x_1}(a) & \frac{\partial f_m}{\partial x_2}(a) & \dots & \frac{\partial f_m}{\partial x_n}(a) \end{pmatrix} \\ d_af(h) = Jac_a(f) \begin{pmatrix} h_1 \\ \vdots \\ h_n \end{pmatrix} &= \left(\sum_{i=1}^n h_i \frac{\partial f_1}{\partial x_i}(a), \sum_{i=1}^n h_i \frac{\partial f_2}{\partial x_i}(a), \dots, \sum_{i=1}^n h_i \frac{\partial f_m}{\partial x_i}(a) \right) \end{aligned}$$

2) Let $f : \mathbb{R}^n \rightarrow \mathbb{R}$ such that all second partial derivatives exist at a point a . The square matrix

$$Hess_a(f) = \begin{pmatrix} \frac{\partial^2 f}{\partial x_1^2}(a) & \frac{\partial^2 f}{\partial x_1 \partial x_2}(a) & \dots & \frac{\partial^2 f}{\partial x_1 \partial x_n}(a) \\ \frac{\partial^2 f}{\partial x_2 \partial x_1}(a) & \frac{\partial^2 f}{\partial x_2^2}(a) & \dots & \frac{\partial^2 f}{\partial x_2 \partial x_n}(a) \\ \vdots & \vdots & \ddots & \vdots \\ \frac{\partial^2 f}{\partial x_n \partial x_1}(a) & \frac{\partial^2 f}{\partial x_n \partial x_2}(a) & \dots & \frac{\partial^2 f}{\partial x_n^2}(a) \end{pmatrix}$$

is called the Hessian matrix of f at a .

Remark: $n = m = 1 \quad f : \mathbb{R} \rightarrow \mathbb{R}$

$$Jac_a(f) = (f'(a)) \quad Hess_a(f) = (f''(a)) = \frac{d^2 f}{dx^2}(a)$$

Corollary Chain rule:

$$Jac_a(g \circ f) = Jac_{f(a)}(g) \times Jac_a(f)$$

Example

$$\begin{aligned} z : \mathbb{R} &\xrightarrow{\gamma} \mathbb{R}^2 \xrightarrow{f} \mathbb{R} \\ t &\mapsto (x(t), y(t)) \xrightarrow{f} f(x(t), y(t)) = z(t) \\ Jac_{(x,y)}f &= \left(\frac{\partial f}{\partial x}(x, y), \frac{\partial f}{\partial y}(x, y) \right); \quad Jac_t(\gamma) = \begin{pmatrix} x'(t) \\ y'(t) \end{pmatrix} \\ Jac_t(z) &= (z'(t)) = \left(\frac{\partial f}{\partial x}(\gamma(t)), \frac{\partial f}{\partial y}(\gamma(t)) \right) \begin{pmatrix} x'(t) \\ y'(t) \end{pmatrix} \\ &= x'(t) \frac{\partial f}{\partial x}(\gamma(t)) + y'(t) \frac{\partial f}{\partial y}(\gamma(t)) \\ \text{So: } \frac{dz}{dt}(t) &= \frac{dx}{dt}(t) \frac{\partial f}{\partial x}(x(t), y(t)) + \frac{dy}{dt}(t) \frac{\partial f}{\partial y}(x(t), y(t)) \end{aligned}$$

In the case of 3 variables:

$$\frac{dw}{dt} = \frac{dx}{dt} \frac{\partial f}{\partial x} + \frac{dy}{dt} \frac{\partial f}{\partial y} + \frac{dz}{dt} \frac{\partial f}{\partial z}$$

$$\begin{aligned} \mathbb{R}^2 &\xrightarrow{\varphi} \mathbb{R}^2 \xrightarrow{f} \mathbb{R} \\ (t, s) &\mapsto (x(t, s), y(t, s)) \mapsto f \circ \varphi(t, s) = w(t, s) \end{aligned}$$

$$\begin{cases} \frac{\partial w}{\partial t} = \frac{\partial x}{\partial t} \frac{\partial f}{\partial x} + \frac{\partial y}{\partial t} \frac{\partial f}{\partial y} \\ \frac{\partial w}{\partial s} = \frac{\partial x}{\partial s} \frac{\partial f}{\partial x} + \frac{\partial y}{\partial s} \frac{\partial f}{\partial y} \end{cases}$$

$$\begin{aligned} \mathbb{R}^2 &\xrightarrow{\varphi} \mathbb{R}^3 \xrightarrow{f} \mathbb{R} \\ (t, s) &\mapsto (x(t, s), y(t, s), z(t, s)) \mapsto f \circ \varphi(t, s) = w(t, s) \end{aligned}$$

$$\begin{cases} \frac{\partial w}{\partial t} = \frac{\partial x}{\partial t} \frac{\partial f}{\partial x} + \frac{\partial y}{\partial t} \frac{\partial f}{\partial y} + \frac{\partial z}{\partial t} \frac{\partial f}{\partial z} \\ \frac{\partial w}{\partial s} = \frac{\partial x}{\partial s} \frac{\partial f}{\partial x} + \frac{\partial y}{\partial s} \frac{\partial f}{\partial y} + \frac{\partial z}{\partial s} \frac{\partial f}{\partial z} \end{cases}$$

Example:

$$\begin{aligned} \varphi(t) &= (t^2 - 2t, t^3) \\ f(x, y) &= x^2 + 2yx \end{aligned}$$

$$\begin{cases} x(t) = t^2 - 2t \\ y(t) = t^3 \end{cases} \quad \begin{cases} \frac{\partial f}{\partial x}(x, y) = 2x + 2y = 2(x + y) \\ \frac{\partial f}{\partial y}(x, y) = 2x \end{cases}$$

$$\begin{aligned} z(t) &= (f \circ \varphi)(t) = (t^2 - 2t)^2 + 2t^3(t^2 - 2t) \\ &= t^4 - 4t^3 + 4t^2 + 2t^5 - 4t^4 \\ &= 2t^5 - 3t^4 - 4t^3 + 4t^2 \\ z'(t) &= 10t^4 - 12t^3 - 12t^2 + 8t \end{aligned}$$

Using chain rule:

$$\begin{aligned} z'(t) &= x'(t) [2(x(t) + y(t))] + y'(t) \cdot 2x(t) \\ &= (2t - 2) \cdot 2(t^2 - 2t + t^3) + 3t^2 \cdot 2(t^2 - 2t) \\ &= (2t - 2)(2t^3 + 2t^2 - 4t) + 6t^2(t^2 - 2t) \\ &= 4t^4 + 4t^3 - 8t^2 - 4t^3 - 4t^2 + 8t + 6t^4 - 12t^3 \\ &= 10t^4 - 12t^3 - 12t^2 + 8t \end{aligned}$$

4 Extrema of function from \mathbb{R}^2 to \mathbb{R}

4.1 Taylor expansion of $f : \mathbb{R}^2 \rightarrow \mathbb{R}$

Definition 17. Let $f : \mathbb{R}^2 \rightarrow \mathbb{R}$ of class C^{p+1} at (a, b) . The Taylor polynomial function of f at (a, b) of degree p is denoted by $T_{(a,b)}^p f$ and is defined as the Taylor polynomial function of degree p at 0 of the function

$$\varphi : \mathbb{R} \rightarrow \mathbb{R}$$

$$t \mapsto f(a + t(x - a), b + t(y - b))$$

evaluated at $t = 1$:

$$\begin{aligned} T_{(a,b)}^p f(x, y) &:= T_0^p \varphi(1) = \sum_{i=0}^p \frac{1}{i!} \varphi^{(i)}(0) \\ &= \varphi(0) + \frac{\varphi'(0)}{1!} + \frac{\varphi''(0)}{2!} + \dots + \frac{\varphi^{(p)}(0)}{p!} \end{aligned}$$

$$\begin{aligned} T_{(a,b)}^p f(x, y) &= \sum_{i=0}^p \frac{1}{i!} \left[\sum_{k=0}^i \binom{i}{k} \frac{\partial^i f}{\partial x^k \partial y^{i-k}}(a, b) (x - a)^k (y - b)^{i-k} \right] \\ &= f(a, b) + (x - a) \frac{\partial f}{\partial x}(a, b) + (y - b) \frac{\partial f}{\partial y}(a, b) \\ &\quad + \frac{1}{2} \left[(x - a)^2 \frac{\partial^2 f}{\partial x^2}(a, b) + 2(x - a)(y - b) \frac{\partial^2 f}{\partial x \partial y}(a, b) + (y - b)^2 \frac{\partial^2 f}{\partial y^2}(a, b) \right] + \dots \end{aligned}$$

$$\begin{aligned}
& \begin{cases} x(t) = a + t(x - a); & y(t) = b + t(y - b) \\ \varphi(t) = f(x(t), y(t)) \end{cases} \\
& \varphi(0) = f(a + 0(x - a), b + 0(y - b)) = f(a, b) \\
& \varphi'(t) = x'(t) \frac{\partial f}{\partial x}(x(t), y(t)) + y'(t) \frac{\partial f}{\partial y}(x(t), y(t)) \\
& \varphi'(t) = (x - a) \frac{\partial f}{\partial x}(x(t), y(t)) + (y - b) \frac{\partial f}{\partial y}(x(t), y(t)) \\
& \varphi''(t) = (x - a) \left[x'(t) \frac{\partial^2 f}{\partial x \partial x}(x(t), y(t)) + y'(t) \frac{\partial^2 f}{\partial x \partial y}(x(t), y(t)) \right] \\
& \quad + (y - b) \left[x'(t) \frac{\partial^2 f}{\partial y \partial x}(x(t), y(t)) + y'(t) \frac{\partial^2 f}{\partial y \partial y}(x(t), y(t)) \right] \\
& \quad \vdots
\end{aligned}$$

Definition 18. *Taylor expansion of $f : \mathbb{R}^2 \rightarrow \mathbb{R}$*

$$f(x, y) = T_{(a,b)}^p f(x, y) + [(x - a)^2 + (y - b)^2]^{p/2} \epsilon_{(a,b)}(x, y)$$

where $\lim_{(x,y) \rightarrow (a,b)} \epsilon_{(a,b)}(x, y) = 0$

Example:

$$f(x, y) = e^{x+y}$$

$$\varphi(t) = f(0 + t(x - 0), 0 + t(y - 0)) = f(tx, ty) = e^{t(x+y)} = e^{t(x+y)}$$

Taylor expansion at $(0, 0)$:

$$f(x, y) = 1 + (x + y) + \frac{1}{2}(x + y)^2 + \frac{1}{6}(x + y)^3 + \dots$$

4.2 Absolute and relative extrema

Definition 19. *Let $f : \mathbb{R}^2 \rightarrow \mathbb{R}$ and $(a, b) \in \text{Dom}(f)$; $D \subset \text{Dom}(f)$*

1) *We say that $f(a, b)$ is a relative maximum of f if there exists an open subset V with $(a, b) \in V \subset D$ and $f(a, b) \geq f(x, y)$ for all $(x, y) \in V$.*

2) *We say that $f(a, b)$ is a relative minimum of f if there exists an open subset V with $(a, b) \in V \subset D$ and $f(a, b) \leq f(x, y)$ for all $(x, y) \in V$.*

3) *In the two cases above, $f(a, b)$ is a relative extremum of f .*

4) *If $V = D$; $f(a, b)$ is an absolute extremum of f on D .*

Definition 20. *Critical points*

$(a, b) \in \text{Dom}(f)$ is a critical point of f if one of the conditions is verified:

$$1) \frac{\partial f}{\partial x}(a, b) = 0 \quad \text{and} \quad \frac{\partial f}{\partial y}(a, b) = 0 \quad (\text{or } d_{(a,b)}f = 0)$$

$$2) \frac{\partial f}{\partial x}(a, b) \text{ or } \frac{\partial f}{\partial y}(a, b) \text{ doesn't exist}$$

Proposition: First order test

If $f(a, b)$ is a relative extremum of f and f is differentiable at (a, b) , then (a, b) is a critical point of f , that is:

$$\frac{\partial f}{\partial x}(a, b) = 0 \text{ and } \frac{\partial f}{\partial y}(a, b) = 0$$

Proof:

Suppose that $f(a, b)$ is a relative minimum of f ;

$$\begin{aligned} & \exists V \text{ such that } f(a, b) \leq f(x, y) \quad \forall (x, y) \in V \\ & \Leftrightarrow f(x, y) - f(a, b) \geq 0 \\ & \exists \delta > 0; (a + h, b) \in V \text{ for all } |h| < \delta; -\delta < h < \delta \\ & f(a + h, b) - f(a, b) \geq 0 \\ & \begin{cases} \frac{f(a+h,b)-f(a,b)}{h} \leq 0, & -\delta < h < 0 \\ \frac{f(a+h,b)-f(a,b)}{h} \geq 0, & 0 < h < \delta \end{cases} \end{aligned}$$

Taking limits:

$$\begin{cases} \lim_{h \rightarrow 0^-} \frac{f(a+h,b)-f(a,b)}{h} = \frac{\partial f}{\partial x}(a, b) \leq 0 \\ \lim_{h \rightarrow 0^+} \frac{f(a+h,b)-f(a,b)}{h} = \frac{\partial f}{\partial x}(a, b) \geq 0 \end{cases} \Rightarrow \frac{\partial f}{\partial x}(a, b) = 0$$

With the same method, we prove that $\frac{\partial f}{\partial y}(a, b) = 0$.

Remark: If (a, b) is a critical point of f ; $f(a, b)$ is not necessarily a relative extremum.

For example:

$$f(x, y) = x^2 - y^2$$

$$\frac{\partial f}{\partial x}(0, 0) = 0 \text{ and } \frac{\partial f}{\partial y}(0, 0) = 0$$

$f(0, 0) = 0$ is not a relative extremum because:

$$\begin{cases} f(x, 0) = x^2 > 0, & \forall x \neq 0 \Rightarrow f(0, 0) \text{ is not maximum} \\ f(0, y) = -y^2 < 0, & \forall y \neq 0 \Rightarrow f(0, 0) \text{ is not minimum} \end{cases}$$

Theorem 3. Second order test

Let $f : \mathbb{R}^2 \rightarrow \mathbb{R}$ and $(a, b) \in \text{Dom}(f)$ such that f is of class C^2 at (a, b) and (a, b) is a critical point of f .

$$\text{Let } \Delta_0 = \frac{\partial^2 f}{\partial x^2}(a, b) \frac{\partial^2 f}{\partial y^2}(a, b) - \left[\frac{\partial^2 f}{\partial x \partial y}(a, b) \right]^2$$

We have:

1) If $\Delta_0 > 0$ and $\frac{\partial^2 f}{\partial x^2}(a, b) > 0$, then $f(a, b)$ is a relative minimum

2) If $\Delta_0 > 0$ and $\frac{\partial^2 f}{\partial x^2}(a, b) < 0$, then $f(a, b)$ is a relative maximum

3) If $\Delta_0 < 0$ $(a, b, f(a, b))$ is a "saddle" point of graph of f

$(f(a, b))$ is not a relative extremum of f

4) If $\Delta_0 = 0$ the test is not conclusive

Proof: Let $A = \frac{\partial^2 f}{\partial x^2}(a, b)$; $B = \frac{\partial^2 f}{\partial x \partial y}(a, b)$; $C = \frac{\partial^2 f}{\partial y^2}(a, b)$

Using the Taylor expansion of degree 2 at (a, b) :

$$\begin{aligned} f(x, y) &= f(a, b) + (x - a) \frac{\partial f}{\partial x}(a, b) + (y - b) \frac{\partial f}{\partial y}(a, b) \\ &\quad + \frac{1}{2} [A(x - a)^2 + 2B(x - a)(y - b) + C(y - b)^2] + o((x - a)^2 + (y - b)^2) \end{aligned}$$

Since (a, b) is a critical point:

$$f(x, y) - f(a, b) = \frac{1}{2} [A(x - a)^2 + 2B(x - a)(y - b) + C(y - b)^2] + o((x - a)^2 + (y - b)^2)$$

Completing the square:

$$\begin{aligned} &A(x - a)^2 + 2B(x - a)(y - b) + C(y - b)^2 \\ &= A \left[(x - a)^2 + 2 \frac{B}{A} (x - a)(y - b) + \frac{C}{A} (y - b)^2 \right] \\ &= A \left[\left(x - a + \frac{B}{A} (y - b) \right)^2 + \left(\frac{C}{A} - \frac{B^2}{A^2} \right) (y - b)^2 \right] \\ &= A \left[\left(x - a + \frac{B}{A} (y - b) \right)^2 + \frac{\Delta_0}{A^2} (y - b)^2 \right] \end{aligned}$$

The sign depends on A and Δ_0 .

Example:

Exercise 09: 1)

$$\begin{aligned} f(x, y) &= 8 - (x - 1)^2 - (y + 1)^2 \\ &= 8 - [(x - 1)^2 + (y + 1)^2] \end{aligned}$$

$f(1, -1) = 8$ is absolute maximum of f ($8 = \max_{\mathbb{R}^2} f$).

f has no minimum, because:

$$\exists (x_n, y_n) = (1, -1 + n) \in \mathbb{R}^2 \text{ such that } \lim_{n \rightarrow +\infty} f(x_n, y_n) = -\infty$$

Using critical points:

$$\begin{cases} \frac{\partial f}{\partial x}(x, y) = -2(x - 1) = 0 \\ \frac{\partial f}{\partial y}(x, y) = -2(y + 1) = 0 \end{cases} \Leftrightarrow \begin{cases} x = 1 \\ y = -1 \end{cases}$$

$$A = -2; B = 0; C = -2; \Delta_0 = 4 > 0 \text{ and } A = -2 < 0$$

So $f(1, -1)$ is a relative maximum.

Since f is C^2 on \mathbb{R}^2 and $(1, -1)$ is the unique critical point, then $f(1, -1)$ is absolute maximum and there is no minimum.

$$2) f(x, y) = \sqrt{4x^2 + y^2 + 4} \geq \sqrt{4} = 2 = f(0, 0), \quad \forall (x, y) \in \mathbb{R}^2$$

Then 2 is absolute minimum of f .

And $\lim_{n \rightarrow +\infty} f(0, n) = +\infty \implies f$ is not upper bounded.

Using critical point tests:

$$\frac{\partial f}{\partial x}(x, y) = \frac{4x}{\sqrt{4x^2 + y^2 + 4}}; \quad \frac{\partial f}{\partial y}(x, y) = \frac{y}{\sqrt{4x^2 + y^2 + 4}}$$

The unique critical point is $(0, 0)$.

Compute second derivatives at $(0, 0)$:

$$\begin{aligned} A &= \lim_{h \rightarrow 0} \frac{\frac{\partial f}{\partial x}(h, 0) - \frac{\partial f}{\partial x}(0, 0)}{h} = \lim_{h \rightarrow 0} \frac{\frac{4h}{\sqrt{4h^2 + 4}} - 0}{h} = 2 \\ B &= \lim_{h \rightarrow 0} \frac{\frac{\partial f}{\partial x}(0, h) - \frac{\partial f}{\partial x}(0, 0)}{h} = 0 \\ C &= \lim_{h \rightarrow 0} \frac{\frac{\partial f}{\partial y}(0, h) - \frac{\partial f}{\partial y}(0, 0)}{h} = \lim_{h \rightarrow 0} \frac{\frac{h}{\sqrt{4 + h^2}} - 0}{h} = \frac{1}{2} \end{aligned}$$

$$\Delta_0 = 2 \cdot \frac{1}{2} - 0^2 = 1 > 0 \text{ and } A = 2 > 0$$

So $f(0, 0)$ is a relative minimum. Since $(0, 0)$ is the unique critical point and f is of class C^2 on \mathbb{R}^2 , then $f(0, 0)$ is absolute minimum and there is no maximum.

3)

$$f(x, y) = 10x + 12y - x^2 - y^2 - 64$$

$$\begin{aligned} f(x, y) &= -64 - [(x^2 - 10x) + (y^2 - 12y)] \\ &= -64 - [(x - 5)^2 - 25 + (y - 6)^2 - 36] \\ &= -64 + 25 + 36 - (x - 5)^2 - (y - 6)^2 \\ &= -3 - (x - 5)^2 - (y - 6)^2 \end{aligned}$$

So $f(5, 6) = -3$ is the absolute maximum, and there is no minimum.